bedrock2/src/FlatToRiscv32Specifics.v
@@ -1,0 +1,17 @@
+Require Import bbv.Word.
+Require Import riscv.util.BitWidths.
+Require Import riscv.Utility.
+Require Import compiler.FlatToRiscvBitWidthSpecifics.
+Require Import riscv.Memory.
+
+
+Instance FlatToRiscv32Specifics(mem: Set)
+         {MW: MachineWidth (word 32)}{IsMem: Memory mem (word 32)}
+  : FlatToRiscvBitWidthSpecifics (word 32) mem := {|
+
+  BitWidth := BW32;
+
+  loadWordwXLEN := loadWord;
+  
+  storeWordwXLEN := storeWord;
+|}.
