bedrock2/src/FlatToRiscv64Proofs.v
@@ -1,0 +1,49 @@
+Require Import compiler.FlatImp.
+Require Import compiler.FlatToRiscvBitWidthSpecificProofs.
+Require Import compiler.FlatToRiscvInvariants.
+Require Import riscv.InstructionCoercions.
+Require Import riscv.AxiomaticRiscv.
+Require Import compiler.util.Common.
+Require Import riscv.Utility.
+Require Import riscv.MachineWidth64.
+Require Import compiler.FlatToRiscv64Specifics.
+Require Import compiler.FlatToRiscvBitWidthSpecifics.
+
+Local Open Scope Z_scope.
+
+
+
+Instance FlatToRiscv64Proofs(mem: Set){IsMem: Memory.Memory mem (word 64)}
+  : FlatToRiscvBitWidthSpecificProofs (word 64) mem.
+Proof.
+  constructor.
+  - intros.
+    unfold containsMem, Memory.write_mem, Memory.read_mem, storeWordwXLEN,
+      loadWordwXLEN, XLEN_in_bytes in *.
+    intros. simpl in *.
+    do 2 (destruct_one_match_hyp; [|discriminate]).
+    inversions H0.
+    destruct_one_match_hyp.
+    + apply weqb_sound in E1. subst.
+      inversions H1.
+      specialize H with (1 := E0).
+      destruct_one_match_hyp; [|discriminate].
+      destruct H as [A B0].
+      split.
+      * apply Memory.loadStoreDouble_eq; try reflexivity.
+        unfold Memory.valid_addr. change (64 / 8) with 8 in *.
+        rewrite Z.eqb_eq in E1.
+        auto.
+      * rewrite Memory.storeDouble_preserves_memSize. assumption.
+    + pose proof H as G.
+      specialize H with (1 := E0). destruct H as [A B].
+      specialize (G addr v0).
+      rewrite E in G. rewrite H1 in G. specialize (G eq_refl). destruct G as [C D].
+      subst.
+      destruct_one_match_hyp; try discriminate.
+      split.
+      * apply weqb_false in E1. change (64 / 8) with 8 in *.
+        rewrite Z.eqb_eq in *.
+        apply @Memory.loadStoreDouble_ne; try congruence; unfold Memory.valid_addr; auto.
+      * rewrite Memory.storeDouble_preserves_memSize. assumption.
+Qed.
