bedrock2/src/FlatToRiscvBitWidthSpecificProofs.v
@@ -1,0 +1,30 @@
+Require Import compiler.FlatImp.
+Require Import compiler.FlatToRiscvBitWidthSpecifics.
+Require Import compiler.FlatToRiscvInvariants.
+Require Import riscv.InstructionCoercions.
+Require Import riscv.AxiomaticRiscv.
+Require Import compiler.util.Common.
+Require Import riscv.Utility.
+
+Local Open Scope Z_scope.
+
+
+Section Proofs.
+
+  Variable (mword: Set).
+  Context {MW: MachineWidth mword}.
+
+  Variable (mem: Set).
+  Context {IsMem: Memory.Memory mem mword}.
+  Context {BWS: FlatToRiscvBitWidthSpecifics mword mem}.
+
+  Class FlatToRiscvBitWidthSpecificProofs := {
+    
+    containsMem_write: forall initialL initialH finalH a v,
+      containsMem initialL initialH ->
+      Memory.write_mem a v initialH = Some finalH ->
+      containsMem (storeWordwXLEN initialL a v) finalH;
+  }.
+
+
+End Proofs.
