bedrock2/src/FlatToRiscvInvariants.v
@@ -1,0 +1,29 @@
+Require Import compiler.FlatImp.
+Require Import compiler.FlatToRiscvBitWidthSpecifics.
+Require Import riscv.InstructionCoercions.
+Require Import riscv.AxiomaticRiscv.
+Require Import compiler.util.Common.
+Require Import riscv.Utility.
+
+Local Open Scope ilist_scope.
+Local Open Scope Z_scope.
+
+Set Implicit Arguments.
+
+
+Section Invariants.
+
+  Context {mword: Set}.
+  Context {MW: MachineWidth mword}.
+
+  Add Ring mword_ring : (@regRing mword MW).
+
+  Context {mem: Set}.
+  Context {IsMem: Memory.Memory mem mword}.
+  Context {BWS: FlatToRiscvBitWidthSpecifics mword mem}.
+
+  Definition containsMem(memL: mem)(memH: compiler.Memory.mem): Prop := forall addr v,
+      compiler.Memory.read_mem addr memH = Some v ->
+      loadWordwXLEN memL addr = v /\ regToZ_unsigned addr + XLEN_in_bytes <= Memory.memSize memL.
+
+End Invariants.
